Split proof-relevant and irrelevent terms. The relation still needs work.

basic.v
@@ -1,3 +1,5 @@
+Generalizable All Variables.
+Set Implicit Arguments.
 (* useful tactics for the development *)
 Ltac split_refl eq_dec a := let H:= fresh in destruct (eq_dec a a) as [H|bad]; [clear H|contradict bad]; auto.
 Ltac split_refl2 eq_dec a a' := let H:= fresh in
@@ -8,3 +10,12 @@ Ltac inverts H := inversion H; subst.
 
 Notation "'dec_type' T" := (forall x y : T, {x=y}+{x<>y}) (at level 70, no associativity).
 
+Inductive eqT {A} (x : A) : A -> Type :=
+  reflT : eqT x x.
+
+Inductive InT {A} (x : A) : list A -> Type :=
+| int_first : `{eqT x y -> InT x (y :: l)}
+| int_rest : `{InT x l -> InT x (a :: l)}.
+
+Notation "x '=T' y" := (eqT x y) (at level 75, no associativity).
+Hint Constructors eqT InT.
